Amortized hash non resizing

theories/ub_logic/hash.v
@@ -1,4 +1,5 @@
 From clutch.ub_logic Require Export ub_clutch lib.map.
+Import Hierarchy.
 Set Default Proof Using "Type*".
 
 Module simple_bit_hash.
@@ -160,5 +161,192 @@ Module simple_bit_hash.
       apply (Forall_map (λ p : nat * Z, p.2)) in HForall; auto.
   Qed.
 
+  Section amortized.
+    Variable max_hash_size : nat.
+    Variable Hineq : max_hash_size <= (val_size+1).
+    Program Definition amortized_error : nonnegreal :=
+      mknonnegreal ((max_hash_size + 1)/(2*(val_size + 1)))%R _.
+    Next Obligation.
+      pose proof (pos_INR val_size) as H.
+      pose proof (pos_INR max_hash_size) as H'.
+      apply Rcomplements.Rdiv_le_0_compat; lra.
+    Qed.
 
+    Definition hashfun_amortized f m : iProp Σ :=
+      ∃ (hm : loc) (k : nat) (ε : nonnegreal),
+        ⌜ f = compute_hash_specialized #hm ⌝ ∗
+        ⌜k = size m⌝ ∗
+        ⌜ (ε.(nonneg) = (((max_hash_size + 1) * k)/2 - sum_n_m (λ x, INR x) 0%nat (k-1)) / (val_size + 1))%R⌝ ∗
+        € ε ∗
+        map_list hm ((λ b, LitV (LitInt b)) <$> m) 
+    .
+
+    #[global] Instance timeless_hashfun_amortized f m :
+      Timeless (hashfun_amortized f m).
+    Proof. apply _. Qed.
+
+    Lemma wp_init_hash_amortized E :
+      {{{ True }}}
+      init_hash #() @ E
+      {{{ f, RET f; hashfun_amortized f ∅ }}}.
+    Proof.
+      rewrite /init_hash.
+      iIntros (Φ) "_ HΦ".
+      wp_pures. rewrite /init_hash_state.
+      wp_apply (wp_init_map with "[//]").
+      iIntros (?) "Hm". wp_pures.
+      rewrite /compute_hash. wp_pures.
+      iApply "HΦ". iExists _. rewrite fmap_empty. iFrame.
+      iMod ec_zero.
+      iModIntro. iExists 0%nat, nnreal_zero.
+      repeat (iSplit; [done|]). iFrame.
+      iPureIntro.
+      simpl.
+      replace (sum_n_m _ _ _) with 0; first lra.
+      rewrite sum_n_n. by simpl. 
+    Qed.
+
+    Lemma wp_hashfun_prev_amortized E f m (n : nat) (b : Z) :
+      m !! n = Some b →
+      {{{ hashfun_amortized f m }}}
+        f #n @ E
+        {{{ RET #b; hashfun_amortized f m }}}.
+    Proof.
+      iIntros (Hlookup Φ) "Hhash HΦ".
+      iDestruct "Hhash" as (hm k ε -> ->) "[% [Hε H]]".
+      wp_apply (wp_hashfun_prev with "[H]"); first done.
+      - iExists _. by iFrame.
+      - iIntros "(%&%&H)". iApply "HΦ".
+        iExists _,_,_. by iFrame.
+    Qed.
+
+    Lemma hashfun_amortized_hashfun f m: ⊢ hashfun_amortized f m -∗ hashfun f m.
+    Proof.
+      iIntros "(%&%&%&->&->&%&He&H)".
+      iExists _; by iFrame.
+    Qed.
+
+    Lemma amortized_inequality (k : nat):
+      (k <= max_hash_size)%nat ->
+      0 <= ((max_hash_size + 1) * k / 2 - sum_n_m (λ x : nat, INR x) 0 (k - 1)) / (val_size + 1).
+    Proof.
+      intros H.
+      pose proof (pos_INR max_hash_size) as H1.
+      pose proof (pos_INR val_size) as H2.    
+      pose proof (pos_INR k) as H3.    
+      apply Rcomplements.Rdiv_le_0_compat; last lra.
+      assert (sum_n_m (λ x : nat, INR x) 0 (k - 1) = (k-1)*k/2) as ->.
+      - clear.
+        induction k.
+        + simpl. rewrite sum_n_n.
+          rewrite Rmult_0_r. by assert (0/2 = 0) as -> by lra.
+        + clear. induction k.
+          * simpl. rewrite sum_n_n.
+            replace (_-_) with 0 by lra.
+            rewrite Rmult_0_l. by assert (0/2 = 0) as -> by lra.
+          * assert (S (S k) - 1 = S (S k - 1))%nat as -> by lia.
+            rewrite sum_n_Sm; last lia.
+            rewrite IHk.
+            replace (plus _ _) with (((S k - 1) * S k / 2) + (S (S k - 1))) by done.
+            assert (∀ k, (INR (S k) - 1) = (INR k)) as H'.
+            { intros. simpl. case_match; first replace (1 - 1) with 0 by lra.
+              - done.
+              - by replace (_+1-1) with (INR (S n)) by lra.
+            }
+            rewrite !H'.
+            replace (S k - 1)%nat with (k)%nat by lia.
+            assert (k * (S k) + S k + S k = S k * S (S k)); last lra.
+            assert (k * S k + S k + S k = S k * (k+1+1)) as ->; try lra.
+            assert (k+1+1 = S (S k)).
+            -- rewrite !S_INR. lra.
+            -- by rewrite H. 
+      - rewrite -!Rmult_minus_distr_r.
+        apply Rcomplements.Rdiv_le_0_compat; try lra.
+        apply Rmult_le_pos; try lra.
+        assert (INR k <= INR max_hash_size); try lra.
+        by apply le_INR.
+    Qed.
+    
+
+    Lemma wp_insert_no_coll_amortized E f m (n : nat) (z : Z) :
+      m !! n = None →
+      (size m < max_hash_size)%nat ->
+      {{{ hashfun_amortized f m ∗ € amortized_error ∗
+          ⌜coll_free m⌝ }}}
+        f #n @ E
+        {{{ (v : Z), RET #v; hashfun_amortized f (<[ n := v ]>m) ∗ ⌜coll_free (<[ n := v ]>m)⌝ }}}.
+    Proof.
+      iIntros (Hlookup Hsize Φ) "(Hhash & Herr & %Hcoll) HΦ".
+      iDestruct "Hhash" as (hm k ε -> ->) "[% [Hε H]]".
+      iAssert (€ (nnreal_div (nnreal_nat (size m)) (nnreal_nat (val_size + 1))) ∗
+               € (mknonnegreal (((max_hash_size + 1) * size (<[n:=0%Z]> m) / 2 - sum_n_m (λ x, INR x) 0%nat (size (<[n:=0%Z]> m) - 1)) / (val_size + 1)) _ )
+              )%I with "[Hε Herr]" as "[Hε Herr]".
+      - iApply ec_split.
+        iCombine "Hε Herr" as "H".
+        iApply (ec_spend_irrel with "[$]").
+        simpl. rewrite H. rewrite map_size_insert_None; [|done].
+        remember (size m) as k.
+        remember (val_size + 1) as v.
+        remember (max_hash_size) as h.
+        assert (∀ x y, x/y = x*/y) as Hdiv.
+        { intros. lra. }
+        destruct k.
+        + simpl. rewrite sum_n_n. rewrite Rmult_0_l Rmult_0_r.
+          replace (INR 0%nat) with 0; last done.
+          rewrite !Rminus_0_r.
+          replace (0/_/_) with 0; last lra.
+          rewrite !Rplus_0_l.
+          rewrite Rmult_1_r.
+          rewrite !Hdiv.
+          rewrite Rinv_mult.
+          lra. 
+        + assert (forall k, S k - 1 = k)%nat as H' by lia.
+          rewrite !H'.
+          clear H'.
+          rewrite sum_n_Sm; last lia.
+          replace (plus _ (INR (S k))) with ((sum_n_m (λ x : nat, INR x) 0 k) + (S k)) by done.
+          rewrite !Hdiv.
+          rewrite !Rmult_minus_distr_r.
+          rewrite (Rmult_plus_distr_r (sum_n_m _ _ _)).
+          rewrite -!Rplus_assoc.
+          rewrite Ropp_plus_distr.
+          rewrite -!Rplus_assoc.
+          assert ((h + 1) * S k * / 2 * / v+ (h + 1) * / (2 * v) = S k * / (val_size + 1)%nat + (h + 1) * S (S k) * / 2 * / v  + - (S k * / v)); try lra.
+          replace (INR((_+_)%nat)) with v; last first.
+          { rewrite Heqv. rewrite -S_INR. f_equal. lia. }
+          assert ( (h + 1) * S k * / 2 * / v + (h + 1) * / (2 * v) = (h + 1) * S (S k) * / 2 * / v); try lra.
+          replace (_*_*_*_) with ((h+1) * (S k) * /(2*v)); last first.
+          { rewrite Rinv_mult. lra. }
+          replace (_*_*_*_) with ((h+1) * (S(S k)) * /(2*v)); last first.
+          { rewrite Rinv_mult. lra. }
+          rewrite -Rdiv_plus_distr.
+          rewrite Hdiv.
+          f_equal.
+          rewrite -{2}(Rmult_1_r (h+1)).
+          rewrite -Rmult_plus_distr_l.
+          f_equal.
+      - wp_apply (wp_insert_no_coll with "[H Hε]"); [done|done|..].
+        + iFrame. iSplitL; try done.
+          iExists _. by iFrame.
+        + iIntros (v) "[H %]".
+          iApply "HΦ".
+          iSplitL; last done.
+          iExists _, _, _. iFrame.
+          repeat (iSplitR); try done.
+          * iPureIntro. simpl. do 3 f_equal.
+            all: by repeat rewrite map_size_insert.
+          * iDestruct "H" as "[% [% H]]".
+            inversion H1; subst.
+            iFrame.
+            Unshelve.
+            apply amortized_inequality.
+            rewrite map_size_insert.
+            case_match => /=; lia.
+    Qed.
+
+  End amortized.
+
+  
 End simple_bit_hash.
+
+
